src/Pyrosome/Lang/SimpleVSubst.v
@@ -22,16 +22,11 @@ Notation subst := (@subst string).
 Notation rule := (@rule string).
 Notation lang := (@lang string).
 
-
-
-Definition value_subst : lang := val_subst ++[("ty",sort_rule [] [])].
-Definition value_subst_def := val_subst_def ++[("ty",sort_rule [] [])].
-
-(*TODO: duplicated*)
-Lemma value_subst_wf : elab_lang_ext [] value_subst_def value_subst.
-Proof. auto_elab. Qed.
+Export Pyrosome.Lang.PolySubst
+  (value_subst, value_subst_def, value_subst_wf,
+    block_subst, block_subst_def, block_subst_wf).
 #[export] Hint Resolve value_subst_wf : elab_pfs.
-
+#[export] Hint Resolve block_subst_wf : elab_pfs.
 
 
 Definition exp_subst : lang := exp_ret ++ exp_subst_base.
@@ -41,14 +36,3 @@ Definition exp_subst_def := exp_ret_def ++ exp_subst_base_def.
 Lemma exp_subst_wf : elab_lang_ext value_subst exp_subst_def exp_subst.
 Proof. auto_elab. Qed.
 #[export] Hint Resolve exp_subst_wf : elab_pfs.
-
-
-
-Definition block_subst_def : lang := block_subst_def.
-Definition block_subst : lang := block_subst.
-
-Definition block_subst_wf
-  : elab_lang_ext value_subst block_subst_def block_subst :=
-  block_subst_wf.
-#[export] Hint Resolve block_subst_wf : elab_pfs.
-
